Fix: Insertion and replacement not handled correctly
Now the function inserting an element into a red black tree
gets a replace flag indicating whether an equivalent element
shall be replace by the element to be inserted or that the
element to be inserted will be inserted at the end of all
equivalent elements.

Therefore only one 'compare3' decider is necessary in sortable
elements. 'compare3 a b' returns either 'LT' with a proof of
'a <= b' and '~ b <= a' or 'EQV' with a proof of 'a <= b' and
'b <= a' or 'GT' with a proof of 'b <= a' and '~ a <= b'.

The 'Inserted.R' relation has been augmented by a replace flag
indicating if replacement or insertion shall happen.

	modified:   src/lib/Binary_search_tree.v
	modified:   src/lib/Core.v
	modified:   src/lib/Red_black_tree.v

src/lib/Red_black_tree.v
@@ -579,22 +579,23 @@ Module Make (S0:SORTABLE).
   (*  ---------------------------------------- *)
   Module Insertion.
     Module Red_black_inserted.
-      (** [R e t u] means that the element [e] has been inserted into the tree
-      [t] resulting in the red black tree [u]. Note that both [t] and [u] must
-      be sorted because of the definition of the [Inserted.R] relation of the
-      module [Binary_search_tree]. *)
-      Inductive R (e:S.t) (t u: Tree.t): Prop :=
+      (** [R e r t u] means that the element [e] has been inserted into the
+      tree [t] or has replaced an equivalent (depending on the replace flag
+      [r]) resulting in the red black tree [u]. Note that both [t] and [u]
+      must be sorted because of the definition of the [Inserted.R] relation of
+      the module [Binary_search_tree]. *)
+      Inductive R (e:S.t) (r:bool) (t u: Tree.t): Prop :=
         make:
           forall h c,
             Red_black.R h c u ->
-            Inserted.R e t u ->
-            R e t u.
+            Inserted.R e r t u ->
+            R e r t u.
     End Red_black_inserted.
 
 
     (** Result type of the insertion function. *)
-    Definition result (e:S.t) (t:Tree.t): Type :=
-      {u:Tree.t | Red_black_inserted.R e t u}.
+    Definition result (e:S.t) (r:bool) (t:Tree.t): Type :=
+      {u:Tree.t | Red_black_inserted.R e r t u}.
 
 
     (** Insertion always starts at a leaf node. An insertion into a leaf node
@@ -612,17 +613,17 @@ Module Make (S0:SORTABLE).
     of the insertion process.*)
 
     Module Red_red.
-    (** [Red_red.R e t a x b y c] means that [e] has been inserted into the
-      valid red black tree [t] but the result has a red red violation. The
-      trees [a], [b] and [c] are black and have the same black height as the
-      original tree [t]. Such a violation can occur only if the original tree
-      [t] is red.*)(**<<
+    (** [Red_red.R e r t a x b y c] means that [e] has been inserted into the
+      valid red black tree [t] (or has replaced an equivalent) but the result
+      has a red red violation. The trees [a], [b] and [c] are black and have
+      the same black height as the original tree [t]. Such a violation can
+      occur only if the original tree [t] is red.*)(**<<
                 yR
              xR    c
            a    b
 >>*)
       Inductive R
-                (e:S.t) (t:Tree.t)
+                (e:S.t) (r:bool) (t:Tree.t)
                 (a:Tree.t) (x:S.t) (b:Tree.t) (y:S.t) (c:Tree.t): Prop :=
         make:
         forall h,
@@ -630,47 +631,51 @@ Module Make (S0:SORTABLE).
           Red_black.R h Color.Black a ->
           Red_black.R h Color.Black b ->
           Red_black.R h Color.Black c ->
-          Inserted.R e t (Tree.Node Color.Red (Tree.Node Color.Red a x b) y c) ->
-          R e t a x b y c.
+          Inserted.R e r t (Tree.Node Color.Red (Tree.Node Color.Red a x b) y c) ->
+          R e r t a x b y c.
     End Red_red.
 
     Module Red.
-    (** [Red.R e t a x b] means that [e] has been inserted into the valid red
-      black tree [t] and the result is a red tree. The trees [a] and [b] are
-      black and have the same black height as the original tree [t]. The
-      original tree [t] can have any color.*)
+    (** [Red.R e r t a x b] means that [e] has been inserted into the valid
+      red black tree [t] (or has replaced an equivalent element) and the
+      result is a red tree. The trees [a] and [b] are black and have the same
+      black height as the original tree [t]. The original tree [t] can have
+      any color.*)
 (**<<
              xR
            a    b
 >>*)
-      Inductive R (e:S.t) (t:Tree.t) (a:Tree.t) (x:S.t) (b:Tree.t): Prop :=
+      Inductive R (e:S.t) (r:bool) (t:Tree.t)
+                (a:Tree.t) (x:S.t) (b:Tree.t): Prop :=
         make:
           forall h c,
             Red_black.R h c t ->
             Red_black.R h Color.Black a ->
             Red_black.R h Color.Black b ->
-            Inserted.R e t (Tree.Node Color.Red a x b) ->
-            R e t a x b.
+            Inserted.R e r t (Tree.Node Color.Red a x b) ->
+            R e r t a x b.
     End Red.
 
     Module Black.
-    (** [Black.R e t a x b] means that [e] has been inserted into the valid
-      red black tree [t] and the result is a black tree. The trees [a] and [b]
-      are black and a black height one less than the original tree [t]. The
-      original tree [t] must be black. Insertion into a red tree cannot result
-      in a black tree without breaking the black height invariant.*)
+    (** [Black.R e r t a x b] means that [e] has been inserted into the valid
+      red black tree [t] (or has replaced an equivalent element) and the
+      result is a black tree. The trees [a] and [b] are black and a black
+      height one less than the original tree [t]. The original tree [t] must
+      be black. Insertion into a red tree cannot result in a black tree
+      without breaking the black height invariant.*)
 (**<<
              xB
            a    b
 >>*)
-      Inductive R (e:S.t) (t:Tree.t) (a:Tree.t) (x:S.t) (b:Tree.t): Prop :=
+      Inductive R (e:S.t) (r:bool) (t:Tree.t)
+                (a:Tree.t) (x:S.t) (b:Tree.t): Prop :=
         make:
           forall h ca cb,
             Red_black.R (S h) Color.Black t ->
             Red_black.R h ca a ->
             Red_black.R h cb b ->
-            Inserted.R e t (Tree.Node Color.Black a x b) ->
-            R e t a x b.
+            Inserted.R e r t (Tree.Node Color.Black a x b) ->
+            R e r t a x b.
     End Black.
 
     (** The intermediate results with a red red violation or a valid red or a
@@ -684,17 +689,17 @@ Module Make (S0:SORTABLE).
          a     b    c                          a     b    c
 >>*)
     Theorem inserted_of_red_red:
-      forall e t a x b y c,
-        Red_red.R e t a x b y c ->
+      forall e r t  a x b y c,
+        Red_red.R e r t a x b y c ->
         Red_black_inserted.R
-          e t
+          e r t
           (Tree.Node
              Color.Black
              (Tree.Node Color.Red a x b)
              y
              c).
     Proof
-      fun e t a x b y c rr =>
+      fun e r t a x b y c rr =>
         match rr with
           Red_red.make rbt rba rbb rbc ins =>
           Red_black_inserted.make
@@ -704,13 +709,13 @@ Module Make (S0:SORTABLE).
 
     (** A red node is already valid. Nothing to be done. *)
     Theorem inserted_of_red:
-      forall e t a x b,
-        Red.R e t a x b ->
+      forall e r t a x b,
+        Red.R e r t a x b ->
         Red_black_inserted.R
-          e t
+          e r t
           (Tree.Node Color.Red a x b).
     Proof
-      fun e t a x b r =>
+      fun e r t a x b r =>
         match r with
           Red.make _ rba rbb ins =>
           Red_black_inserted.make (Red_black.red _ rba rbb) ins
@@ -718,13 +723,13 @@ Module Make (S0:SORTABLE).
 
     (** A black node is already valid. Nothing to be done. *)
     Theorem inserted_of_black:
-      forall e t a x b,
-        Black.R e t a x b ->
+      forall e r t a x b,
+        Black.R e r t a x b ->
         Red_black_inserted.R
-          e t
+          e r t
           (Tree.Node Color.Black a x b).
     Proof
-      fun e t a x b black =>
+      fun e r t a x b black =>
         match black with
           Black.make _ rba rbb ins =>
           Red_black_inserted.make (Red_black.black _ rba rbb) ins
@@ -751,17 +756,18 @@ Module Make (S0:SORTABLE).
     be black because t1 is red. Therefore the resulting tree can have one
     black height level more than t1, a, b and c.*)
     Theorem red_of_left_red_red:
-      forall e cn t1 yn t2 a x b y c,
+      forall e r cn t1 yn t2 a x b y c,
         Red_black_sorted.P (Tree.Node cn t1 yn t2) ->
         e <= yn ->
-        Red_red.R e t1 a x b y c ->
-        Red.R e
+        (yn <= e -> r = false) ->
+        Red_red.R e r t1 a x b y c ->
+        Red.R e r
               (Tree.Node cn t1 yn t2)
               (Tree.Node Color.Black a x b)
               y
               (Tree.Node Color.Black c yn t2).
     Proof
-      fun e cn t1 yn t2 a x b y c rbs eyn rr =>
+      fun e r cn t1 yn t2 a x b y c rbs eyn yner rr =>
         match rr with
           Red_red.make rbt1_0 rba rbb rbc ins1 =>
           Red_black_sorted.use_left_red
@@ -773,7 +779,7 @@ Module Make (S0:SORTABLE).
                      Color.Black
                      (Inserted.rotate_right
                         (Inserted.left
-                           cn Color.Black eyn st1 st2 ins1))
+                           cn Color.Black eyn yner st1 st2 ins1))
                in
                let heq: _ = h := Red_black.black_height_unique rbt1_0 rbt1 in
                let P t h := Red_black.R h _ t in
@@ -802,17 +808,18 @@ Module Make (S0:SORTABLE).
                 b  c
 >>*)
     Theorem red_of_right_red_red:
-      forall e cn t1 yn t2 a x b y c,
+      forall e r cn t1 yn t2 a x b y c,
         Red_black_sorted.P (Tree.Node cn t1 yn t2) ->
         yn <= e ->
-        Red_red.R e t2 a x b y c ->
-        Red.R e
+        (e <= yn -> r = false) ->
+        Red_red.R e r t2 a x b y c ->
+        Red.R e r
               (Tree.Node cn t1 yn t2)
               (Tree.Node Color.Black t1 yn a)
               x
               (Tree.Node Color.Black b y c).
     Proof
-      fun e cn t1 yn t2 a x b y c rbs yne rr =>
+      fun e r cn t1 yn t2 a x b y c rbs yne eynr rr =>
         match rr with
           Red_red.make rbt2_0 rba rbb rbc ins2 =>
           Red_black_sorted.use_right_red
@@ -824,7 +831,7 @@ Module Make (S0:SORTABLE).
                      Color.Black
                      (Inserted.rotate_left
                         (Inserted.right
-                           cn Color.Black yne st1 st2
+                           cn Color.Black yne eynr st1 st2
                            (Inserted.rotate_right ins2))) in
                let heq: _ = h := Red_black.black_height_unique rbt2_0 rbt2 in
                let P t h := Red_black.R h _ t in
@@ -852,15 +859,16 @@ Module Make (S0:SORTABLE).
        a  b
 >>*)
     Theorem red_red_of_left_red:
-      forall e t1 yn t2 a x b,
+      forall e r t1 yn t2 a x b,
         Red_black_sorted.P (Tree.Node Color.Red t1 yn t2) ->
         e <= yn ->
-        Red.R e t1 a x b ->
+        (yn <= e -> r = false) ->
+        Red.R e r t1 a x b ->
         Red_red.R
-          e (Tree.Node Color.Red t1 yn t2)
+          e r (Tree.Node Color.Red t1 yn t2)
           a x b yn t2.
     Proof
-      fun e t1 yn t2 a x b rbst e_yn r =>
+      fun e r t1 yn t2 a x b rbst e_yn yn_e_r r =>
         match r with
           Red.make rbt1_0 rba rbb ins1 =>
           Red_black_sorted.use_red_node
@@ -868,7 +876,7 @@ Module Make (S0:SORTABLE).
             (fun h lo hi rbt1 rbt2 rbt lo_yn yn_hi st1 st2 st =>
                let insu :=
                    Inserted.left
-                     Color.Red Color.Red e_yn st1 st2 ins1 in
+                     Color.Red Color.Red e_yn yn_e_r st1 st2 ins1 in
                let heq: _ = h := Red_black.black_height_unique rbt1_0 rbt1 in
                let P t h := Red_black.R h Color.Black t in
                Red_red.make
@@ -889,15 +897,16 @@ Module Make (S0:SORTABLE).
               a  b                   t1   a
 >>*)
     Theorem red_red_of_right_red:
-      forall e t1 yn t2 a x b,
+      forall e r t1 yn t2 a x b,
         Red_black_sorted.P (Tree.Node Color.Red t1 yn t2) ->
         yn <= e ->
-        Red.R e t2 a x b ->
+        (e <= yn -> r = false) ->
+        Red.R e r t2 a x b ->
         Red_red.R
-          e (Tree.Node Color.Red t1 yn t2)
+          e r (Tree.Node Color.Red t1 yn t2)
           t1 yn a x b.
     Proof
-      fun e t1 yn t2 a x b rbst yn_e r =>
+      fun e r t1 yn t2 a x b rbst yn_e e_yn_r r =>
         match r with
           Red.make rbt2_0 rba rbb ins2 =>
           Red_black_sorted.use_red_node
@@ -906,7 +915,7 @@ Module Make (S0:SORTABLE).
                let insv :=
                    Inserted.rotate_left
                      (Inserted.right
-                        Color.Red Color.Red yn_e st1 st2 ins2) in
+                        Color.Red Color.Red yn_e e_yn_r st1 st2 ins2) in
                let heq: _ = h := Red_black.black_height_unique rbt2_0 rbt2 in
                let P t h := Red_black.R h Color.Black t in
                Red_red.make
@@ -932,17 +941,18 @@ Module Make (S0:SORTABLE).
        a  b
 >>*)
     Theorem black_of_left_red:
-      forall e t1 yn t2 a x b,
+      forall e r t1 yn t2 a x b,
         Red_black_sorted.P (Tree.Node Color.Black t1 yn t2) ->
         e <= yn ->
-        Red.R e t1 a x b ->
+        (yn <= e -> r = false) ->
+        Red.R e r t1 a x b ->
         Black.R
-          e (Tree.Node Color.Black t1 yn t2)
+          e r (Tree.Node Color.Black t1 yn t2)
           (Tree.Node Color.Red a x b)
           yn
           t2.
     Proof
-      fun e t1 yn t2 a x b rbst e_yn red =>
+      fun e r t1 yn t2 a x b rbst e_yn yn_e_r red =>
         match red with
           Red.make rbt1_0 rba rbb ins1 =>
           Red_black_sorted.use_black_node
@@ -958,23 +968,24 @@ Module Make (S0:SORTABLE).
                     (Equal.use heq (P b) rbb))
                  rbt2
                  (Inserted.left
-                    Color.Black Color.Black e_yn st1 st2 ins1)
+                    Color.Black Color.Black e_yn yn_e_r st1 st2 ins1)
             )
         end.
 
     (** Symmetrical situtation for insertion into the right subtree. *)
     Theorem black_of_right_red:
-      forall e t1 yn t2 a x b,
+      forall e r t1 yn t2 a x b,
         Red_black_sorted.P (Tree.Node Color.Black t1 yn t2) ->
         yn <= e ->
-        Red.R e t2 a x b ->
+        (e <= yn -> r = false) ->
+        Red.R e r t2 a x b ->
         Black.R
-          e (Tree.Node Color.Black t1 yn t2)
+          e r (Tree.Node Color.Black t1 yn t2)
           t1
           yn
           (Tree.Node Color.Red a x b).
     Proof
-      fun e t1 yn t2 a x b rbst yn_e red =>
+      fun e r t1 yn t2 a x b rbst yn_e e_yn_r red =>
         match red with
           Red.make rbt2_0 rba rbb ins2 =>
           Red_black_sorted.use_black_node
@@ -990,7 +1001,7 @@ Module Make (S0:SORTABLE).
                     (Equal.use heq (P a) rba)
                     (Equal.use heq (P b) rbb))
                  (Inserted.right
-                    Color.Black Color.Black yn_e st1 st2 ins2)
+                    Color.Black Color.Black yn_e e_yn_r st1 st2 ins2)
             )
         end.
 
@@ -998,17 +1009,18 @@ Module Make (S0:SORTABLE).
     subtree. If the original root is black we can insert the new left black
     subtree.*)
     Theorem black_of_left_black:
-      forall e t1 yn t2 a x b,
+      forall e r t1 yn t2 a x b,
         Red_black_sorted.P (Tree.Node Color.Black t1 yn t2) ->
         e <= yn ->
-        Black.R e t1 a x b ->
+        (yn <= e -> r = false) ->
+        Black.R e r t1 a x b ->
         Black.R
-          e (Tree.Node Color.Black t1 yn t2)
+          e r (Tree.Node Color.Black t1 yn t2)
           (Tree.Node Color.Black a x b)
           yn
           t2.
     Proof
-      fun e t1 yn t2 a x b rbst e_yn black =>
+      fun e r t1 yn t2 a x b rbst e_yn yn_e_r black =>
         match black with
           Black.make rbt1_0 rba rbb ins1 =>
           Red_black_sorted.use_black_node
@@ -1021,7 +1033,7 @@ Module Make (S0:SORTABLE).
                     heq (fun h => Red_black.R h _ _)
                     (Red_black.black x rba rbb))
                  rbt2
-                 (Inserted.left Color.Black Color.Black e_yn st1 st2 ins1)
+                 (Inserted.left Color.Black Color.Black e_yn yn_e_r st1 st2 ins1)
             )
         end.
 
@@ -1029,17 +1041,18 @@ Module Make (S0:SORTABLE).
 
     (** Symmetrical situtation for insertion into the right subtree. *)
     Theorem black_of_right_black:
-      forall e t1 yn t2 a x b,
+      forall e r t1 yn t2 a x b,
         Red_black_sorted.P (Tree.Node Color.Black t1 yn t2) ->
         yn <= e ->
-        Black.R e t2 a x b ->
+        (e <= yn -> r = false) ->
+        Black.R e r t2 a x b ->
         Black.R
-          e (Tree.Node Color.Black t1 yn t2)
+          e r (Tree.Node Color.Black t1 yn t2)
           t1
           yn
           (Tree.Node Color.Black a x b).
     Proof
-      fun e t1 yn t2 a x b rbst yn_e black =>
+      fun e r t1 yn t2 a x b rbst yn_e e_yn_r black =>
         match black with
           Black.make rbt2_0 rba rbb ins2 =>
           Red_black_sorted.use_black_node
@@ -1052,7 +1065,7 @@ Module Make (S0:SORTABLE).
                  (Equal.use
                     heq (fun h => Red_black.R h _ _)
                     (Red_black.black x rba rbb))
-                 (Inserted.right Color.Black Color.Black yn_e st1 st2 ins2)
+                 (Inserted.right Color.Black Color.Black yn_e e_yn_r st1 st2 ins2)
             )
         end.
 
@@ -1062,17 +1075,18 @@ Module Make (S0:SORTABLE).
     subtree. If the original root is red we can insert the new left black
     subtree and the resulting tree stays red. *)
     Theorem red_of_left_black:
-      forall e t1 yn t2 a x b,
+      forall e r t1 yn t2 a x b,
         Red_black_sorted.P (Tree.Node Color.Red t1 yn t2) ->
         e <= yn ->
-        Black.R e t1 a x b ->
+        (yn <= e -> r = false) ->
+        Black.R e r t1 a x b ->
         Red.R
-          e (Tree.Node Color.Red t1 yn t2)
+          e r (Tree.Node Color.Red t1 yn t2)
           (Tree.Node Color.Black a x b)
           yn
           t2.
     Proof
-      fun e t1 yn t2 a x b rbst e_yn black =>
+      fun e r t1 yn t2 a x b rbst e_yn yn_e_r black =>
         match black with
           Black.make rbt1_0 rba rbb ins1 =>
           Red_black_sorted.use_red_node
@@ -1085,24 +1099,25 @@ Module Make (S0:SORTABLE).
                     heq (fun h => Red_black.R h _ _)
                     (Red_black.black x rba rbb))
                  rbt2
-                 (Inserted.left Color.Red Color.Red e_yn st1 st2 ins1)
+                 (Inserted.left Color.Red Color.Red e_yn yn_e_r st1 st2 ins1)
             )
         end.
 
 
     (** Symmetrical situtation for insertion into the right subtree. *)
     Theorem red_of_right_black:
-      forall e t1 yn t2 a x b,
+      forall e r t1 yn t2 a x b,
         Red_black_sorted.P (Tree.Node Color.Red t1 yn t2) ->
         yn <= e ->
-        Black.R e t2 a x b ->
+        (e <= yn -> r = false) ->
+        Black.R e r t2 a x b ->
         Red.R
-          e (Tree.Node Color.Red t1 yn t2)
+          e r (Tree.Node Color.Red t1 yn t2)
           t1
           yn
           (Tree.Node Color.Black a x b).
     Proof
-      fun e t1 yn t2 a x b rbst yn_e black =>
+      fun e r t1 yn t2 a x b rbst yn_e e_yn_r black =>
         match black with
         | Black.make rbt2_0 rba rbb ins2 =>
           Red_black_sorted.use_red_node
@@ -1115,7 +1130,7 @@ Module Make (S0:SORTABLE).
                  (Equal.use
                     heq (fun h => Red_black.R h _ _)
                     (Red_black.black x rba rbb))
-                 (Inserted.right Color.Red Color.Red yn_e st1 st2 ins2)
+                 (Inserted.right Color.Red Color.Red yn_e e_yn_r st1 st2 ins2)
             )
         end.
 
@@ -1123,126 +1138,144 @@ Module Make (S0:SORTABLE).
 
     (** An intermediate insert result is either a red red violation or a valid
     red tree or a valid black tree.*)
-    Inductive result0 (e:S.t) (t:Tree.t): Type :=
+    Inductive result0 (e:S.t) (r:bool) (t:Tree.t): Type :=
     | Red_red:
         forall a x b y c,
-          Red_red.R e t a x b y c ->
-          result0 e t
+          Red_red.R e r t a x b y c ->
+          result0 e r t
     | Red:
         forall a x b,
-          Red.R e t a x b ->
-          result0 e t
+          Red.R e r t a x b ->
+          result0 e r t
     | Black:
         forall a x b,
-          Black.R e t a x b ->
-          result0 e t.
+          Black.R e r t a x b ->
+          result0 e r t.
 
     (** Insertion of a new element [e] into a sorted red black tree [t].*)
-    Fact insert (e:S.t) (t:Tree.t) (rbs:Red_black_sorted.P t): result e t.
+    Fact insert (e:S.t) (r:bool) (t:Tree.t)
+         (rbs:Red_black_sorted.P t): result e r t.
     Proof
       let insert0:
-            forall t,
-              Red_black_sorted.P t -> result0 e t :=
-          fix insert0 t :=
+            forall r t,
+              Red_black_sorted.P t -> result0 e r t :=
+          fix insert0 r t :=
             match t with
 
             | Tree.Leaf =>
               fun _ =>
                 let rbl := Red_black.leaf in
-                Red (Red.make rbl rbl rbl (Inserted.leaf Color.Red e))
+                Red (Red.make rbl rbl rbl (Inserted.leaf Color.Red e r))
 
             | Tree.Node cn t1 yn t2 =>
 
-              match S.compare3 e yn with
-
-              | Relation.LT e_yn =>
-
-                fun rbs =>
-                  (match insert0 t1 (Red_black_sorted.left_son rbs), cn with
+              let insert_left r e_yn (yn_e_r: yn <= e -> r = false) rbs :=
+                  (match insert0 r t1 (Red_black_sorted.left_son rbs), cn with
                    | Red_red red_red, _ =>
 
-                     fun _ => Red (red_of_left_red_red rbs e_yn red_red)
+                     fun _ => Red (red_of_left_red_red rbs e_yn yn_e_r red_red)
 
                    | Red red, Color.Red =>
 
-                     fun rbs => Red_red (red_red_of_left_red rbs e_yn red)
+                     fun rbs => Red_red (red_red_of_left_red rbs e_yn yn_e_r red)
 
                    | Red red, Color.Black =>
 
-                     fun rbs => Black (black_of_left_red rbs e_yn red)
+                     fun rbs => Black (black_of_left_red rbs e_yn yn_e_r red)
 
                    | Black black, Color.Black =>
 
-                     fun rbs => Black (black_of_left_black rbs e_yn black)
+                     fun rbs => Black (black_of_left_black rbs e_yn yn_e_r black)
 
                    | Black black, Color.Red =>
 
-                     fun rbs => Red (red_of_left_black rbs e_yn black)
+                     fun rbs => Red (red_of_left_black rbs e_yn yn_e_r black)
                   end) rbs
-
-              | Relation.EQV e_yn yn_e =>
-
-                match cn with
-
-                | Color.Red =>
-                  fun rbst =>
-                    let red :=
-                        Red_black_sorted.use_red_node
-                          rbst
-                          (fun h lo hi rbt1 rbt2 rbt lo_yn yn_hi st1 st2 st =>
-                             Red.make
-                               rbt rbt1 rbt2
-                               (Inserted.replace
-                                  Color.Red Color.Red
-                                  (conj e_yn yn_e) st1 st2))
-                    in
-                    Red red
-                | Color.Black =>
-
-                  fun rbst =>
-                    let black :=
-                        Red_black_sorted.use_black_node
-                          rbst
-                          (fun h ct1 ct2 lo hi rbt1 rbt2 rbt
-                               lo_yn yn_hi st1 st2 st =>
-                             Black.make
-                               rbt rbt1 rbt2
-                               (Inserted.replace
-                                  Color.Black Color.Black
-                                  (conj e_yn yn_e) st1 st2))
-                    in
-                    Black black
-                end
-
-              | Relation.GT yn_e =>
-
-                fun rbs =>
-                  (match insert0 t2 (Red_black_sorted.right_son rbs), cn with
+              in
+              let insert_right r yn_e (e_yn_r:e <= yn -> r = false) rbs :=
+                  (match insert0 r t2 (Red_black_sorted.right_son rbs), cn with
                    | Red_red red_red, _ =>
 
                      fun _ =>
-                       Red (red_of_right_red_red rbs yn_e red_red)
+                       Red (red_of_right_red_red rbs yn_e e_yn_r red_red)
 
                    | Red red, Color.Red =>
 
-                     fun rbs => Red_red (red_red_of_right_red rbs yn_e red)
+                     fun rbs => Red_red (red_red_of_right_red rbs yn_e e_yn_r red)
 
                    | Red red, Color.Black =>
 
-                     fun rbs => Black (black_of_right_red rbs yn_e red)
+                     fun rbs => Black (black_of_right_red rbs yn_e e_yn_r red)
 
                    | Black black, Color.Red =>
 
-                     fun rbs =>  Red (red_of_right_black rbs yn_e black)
+                     fun rbs =>  Red (red_of_right_black rbs yn_e e_yn_r black)
 
                    | Black black, Color.Black =>
 
-                     fun rbs => Black (black_of_right_black rbs yn_e black)
+                     fun rbs => Black (black_of_right_black rbs yn_e e_yn_r black)
                   end) rbs
+              in
+              let replace r (rtrue:r = true) e_yn yn_e rbst :=
+                  match cn with
+
+                  | Color.Red =>
+                    fun rbst =>
+                      let red :=
+                          Red_black_sorted.use_red_node
+                            rbst
+                            (fun h lo hi rbt1 rbt2 rbt lo_yn yn_hi st1 st2 st =>
+                               Red.make
+                                 rbt rbt1 rbt2
+                                 (Inserted.replace
+                                    Color.Red Color.Red
+                                    (conj e_yn yn_e) rtrue st1 st2))
+                      in
+                      Red red
+                  | Color.Black =>
+
+                    fun rbst =>
+                      let black :=
+                          Red_black_sorted.use_black_node
+                            rbst
+                            (fun h ct1 ct2 lo hi rbt1 rbt2 rbt
+                                 lo_yn yn_hi st1 st2 st =>
+                               Black.make
+                                 rbt rbt1 rbt2
+                                 (Inserted.replace
+                                    Color.Black Color.Black
+                                    (conj e_yn yn_e) rtrue st1 st2))
+                      in
+                      Black black
+                  end
+              in
+
+              match S.compare3 e yn with
+
+              | Relation.LT e_yn not_yn_e =>
+
+                let yn_e_r: yn <= e -> r = false :=
+                    fun yn_e => ex_falso (not_yn_e yn_e) in
+                insert_left r e_yn yn_e_r
+
+              | Relation.EQV e_yn yn_e =>
+
+                match r with
+                | true =>
+                  replace true eq_refl e_yn yn_e rbs
+                | false =>
+                  insert_right false yn_e (fun _ => eq_refl)
+                end
+
+              | Relation.GT yn_e not_e_yn =>
+
+                let e_yn_r: e <= yn -> r = false :=
+                    fun e_yn => ex_falso (not_e_yn e_yn) in
+                insert_right r yn_e e_yn_r
               end
             end
       in
-      match insert0 t rbs with
+      match insert0 r t rbs with
       | Red_red rr =>
         exist _ _ (inserted_of_red_red rr)
       | Red r =>
