src/lib/Core.v
@@ -394,21 +394,14 @@ Module Relation.
     | GE:  R b a -> Comparison2 a b.
 
     Inductive Comparison3 (a b:A): Set :=
-    | LT:  R a b -> Comparison3 a b
-    | EQV: R a b -> R b a  -> Comparison3 a b
-    | GT:  R b a -> Comparison3 a b.
-
-    Inductive Comparison3_strict (a b:A): Set :=
-    | LT_strict:  R a b -> ~ R b a -> Comparison3_strict a b
-    | EQV_strict: R a b -> R b a   -> Comparison3_strict a b
-    | GT_strict:  R b a -> ~ R a b -> Comparison3_strict a b.
+    | LT:  R a b -> ~ R b a -> Comparison3 a b
+    | EQV: R a b -> R b a   -> Comparison3 a b
+    | GT:  R b a -> ~ R a b -> Comparison3 a b.
 
     Definition Comparer2: Type :=
       forall a b:A, Comparison2 a b.
     Definition Comparer3: Type :=
       forall a b:A, Comparison3 a b.
-    Definition Comparer3_strict: Type :=
-      forall a b:A, Comparison3_strict a b.
 
     Theorem comparable2_is_complete:
       forall (c:Comparer2), Complete.
@@ -424,18 +417,15 @@ Module Relation.
     Proof
       fun c a b =>
         match c a b with
-        | LT  p => or_introl p
+        | LT  p _   => or_introl p
         | EQV p1 p2 => or_introl p1
-        | GT  p => or_intror p
+        | GT  p _   => or_intror p
         end.
   End endorelation.
 
   Arguments LT    [_] [_] [_] [_] _.
   Arguments EQV   [_] [_] [_] [_] _ _.
   Arguments GT    [_] [_] [_] [_] _.
-  Arguments LT_strict    [_] [_] [_] [_] _.
-  Arguments EQV_strict   [_] [_] [_] [_] _ _.
-  Arguments GT_strict    [_] [_] [_] [_] _.
   Arguments LE    [_ _ _ _]  _.
   Arguments GE    [_ _ _ _]  _.
 
@@ -535,7 +525,6 @@ Module Type SORTABLE <: ANY.
 
   Parameter compare2: Comparer2 Less_equal.
   Parameter compare3: Comparer3 Less_equal.
-  Parameter compare3_strict: Comparer3_strict Less_equal.
 End SORTABLE.
 
 Module Sortable_plus (S:SORTABLE).
